changed the definition of a procedure and of proc_is_correct

BoogieLang/Ast.thy
@@ -73,11 +73,20 @@ fun find_label :: "label \<Rightarrow> bigblock list \<Rightarrow> cont \<Righta
         else (find_label lbl bbs cont))"
   | "find_label lbl ((BigBlock bb_name cmds (Some s) (Some t)) # bbs) cont = None"
 
+fun get_state :: "'a ast_config \<Rightarrow> 'a state"
+  where
+    "get_state (bb, cont, s1) = s1"
+
+fun is_final :: "'a ast_config \<Rightarrow> bool" 
+  where
+    "is_final ((BigBlock bb_name [] None None), KStop, s1) = True"
+  | "is_final other = False"
+
 text\<open>function defining the semantics of bigblocks; small-step semantics 
       Note: arrow symbols in the 'syntactic sugar' clash if the exact same syntax is used as in red_cmd\<close>
-inductive red_bigblock :: "'a absval_ty_fun \<Rightarrow> proc_context \<Rightarrow> var_context \<Rightarrow> 'a fun_interp \<Rightarrow> rtype_env  \<Rightarrow> ast \<Rightarrow> 'a ast_config \<Rightarrow> 'a ast_config \<Rightarrow> bool" 
+inductive red_bigblock :: "'a absval_ty_fun \<Rightarrow> 'struct_ty proc_context  \<Rightarrow> var_context \<Rightarrow> 'a fun_interp \<Rightarrow> rtype_env  \<Rightarrow> ast \<Rightarrow> 'a ast_config \<Rightarrow> 'a ast_config \<Rightarrow> bool" 
   ("_,_,_,_,_,_ \<turnstile> (\<langle>_\<rangle> \<longrightarrow>/ _)" [51,0,0,0] 81)
-  for A :: "'a absval_ty_fun" and M :: proc_context and \<Lambda> :: var_context and \<Gamma> :: "'a fun_interp" and \<Omega> :: rtype_env and T :: ast
+  for A :: "'a absval_ty_fun" and M :: "'struct_ty proc_context"  and \<Lambda> :: var_context and \<Gamma> :: "'a fun_interp" and \<Omega> :: rtype_env and T :: ast
   where
     RedSimpleCmds: 
     "\<lbrakk>(A,M,\<Lambda>,\<Gamma>,\<Omega> \<turnstile> \<langle>cs, (Normal n_s)\<rangle> [\<rightarrow>] s1) \<and> (cs \<noteq> Nil) \<rbrakk> 
@@ -86,7 +95,7 @@ inductive red_bigblock :: "'a absval_ty_fun \<Rightarrow> proc_context \<Rightar
 
   (* TODO: fix this rule! *)
   | RedFailure_or_Magic: 
-    "\<lbrakk> (s1 = Magic) \<or> (s1 = Failure) \<rbrakk> 
+    "\<lbrakk> (s1 = Magic) \<or> (s1 = Failure); \<not> (is_final ((BigBlock bb_name [] str_cmd tr_cmd), cont0, s1))  \<rbrakk> 
       \<Longrightarrow> A,M,\<Lambda>,\<Gamma>,\<Omega>,T \<turnstile> \<langle>((BigBlock bb_name [] str_cmd tr_cmd), cont0, s1)\<rangle> \<longrightarrow> 
                           ((BigBlock bb_name [] None None), KStop, s1)"
 
@@ -166,40 +175,24 @@ inductive red_bigblock :: "'a absval_ty_fun \<Rightarrow> proc_context \<Rightar
         \<Longrightarrow> A,M,\<Lambda>,\<Gamma>,\<Omega>,T \<turnstile> \<langle>((BigBlock bb_name [] None (Some (Goto label))), cont0, Normal n_s)\<rangle> \<longrightarrow> 
                             (found_bigblock, found_cont, (Normal n_s))"
 
-abbreviation red_bigblock_k_step :: "'a absval_ty_fun \<Rightarrow> proc_context \<Rightarrow> var_context \<Rightarrow> 'a fun_interp \<Rightarrow> rtype_env \<Rightarrow> ast \<Rightarrow> 'a ast_config \<Rightarrow> nat \<Rightarrow> 'a ast_config \<Rightarrow> bool"
+abbreviation red_bigblock_k_step :: "'a absval_ty_fun \<Rightarrow> 'struct_ty  proc_context \<Rightarrow> var_context \<Rightarrow> 'a fun_interp \<Rightarrow> rtype_env \<Rightarrow> ast \<Rightarrow> 'a ast_config \<Rightarrow> nat \<Rightarrow> 'a ast_config \<Rightarrow> bool"
   ("_,_,_,_,_,_ \<turnstile>_ -n\<longrightarrow>^_/ _" [51,0,0,0,0] 81)
 where "red_bigblock_k_step A M \<Lambda> \<Gamma> \<Omega> T c1 n c2 \<equiv> ((red_bigblock A M \<Lambda> \<Gamma> \<Omega> T)^^n) c1 c2"
-
-(*
-inductive red_bigblock_trans :: "'a absval_ty_fun \<Rightarrow> proc_context \<Rightarrow> var_context \<Rightarrow> 'a fun_interp \<Rightarrow> rtype_env  \<Rightarrow> ast \<Rightarrow> 'a ast_config \<Rightarrow> 'a ast_config \<Rightarrow> bool" 
-  ("_,_,_,_,_,_ \<turnstile> (\<langle>_\<rangle> [\<longrightarrow>]/ _)" [51,0,0,0] 81)
-  for A :: "'a absval_ty_fun" and M :: proc_context and \<Lambda> :: var_context and \<Gamma> :: "'a fun_interp" and \<Omega> :: rtype_env and T :: ast
-  where
-    BBRefl: "A,M,\<Lambda>,\<Gamma>,\<Omega>,T \<turnstile> \<langle>config\<rangle> [\<longrightarrow>] config"
-  | BBTrans: "\<lbrakk> A,M,\<Lambda>,\<Gamma>,\<Omega>,T \<turnstile> \<langle>start_config\<rangle> \<longrightarrow> inter_config;  A,M,\<Lambda>,\<Gamma>,\<Omega>,T \<turnstile> \<langle>inter_config\<rangle> [\<longrightarrow>] end_config\<rbrakk> \<Longrightarrow> A,M,\<Lambda>,\<Gamma>,\<Omega>,T \<turnstile> \<langle>start_config\<rangle> [\<longrightarrow>] end_config"
-*)
 
 subsection \<open>Procedure Correctness\<close>
 
 text\<open>defining correctness of the AST\<close>
 
-record ast_procedure =
+(*
+record 'struct_ty ast_procedure =
   proc_ty_args :: nat
   proc_args :: vdecls
   proc_rets :: vdecls
   proc_modifs :: "vname list"
   proc_pres :: "(expr \<times> bool) list" 
   proc_posts :: "(expr \<times> bool) list"
-  proc_body :: "(vdecls \<times> ast) option"
-
-fun get_state :: "'a ast_config \<Rightarrow> 'a state"
-  where
-    "get_state (bb, cont, s1) = s1"
-
-fun is_final :: "'a ast_config \<Rightarrow> bool" 
-  where
-    "is_final ((BigBlock bb_name [] None None), KStop, s1) = True"
-  | "is_final other = False"
+  proc_body :: "(vdecls \<times> 'struct_ty) option"
+*)
 
 fun init_ast :: "ast \<Rightarrow> 'a nstate \<Rightarrow> 'a ast_config"
   where
@@ -211,18 +204,19 @@ definition valid_configuration
          (get_state (bb, cont, state)) \<noteq> Failure \<and> 
          (is_final (bb, cont, state) \<longrightarrow> (\<forall>ns'. (get_state (bb, cont, state)) = Normal ns' \<longrightarrow> expr_all_sat A \<Lambda> \<Gamma> \<Omega> ns' posts))"
 
-definition proc_body_satisfies_spec :: "'a absval_ty_fun \<Rightarrow> proc_context \<Rightarrow> var_context \<Rightarrow> 'a fun_interp \<Rightarrow> rtype_env \<Rightarrow> expr list \<Rightarrow> expr list \<Rightarrow> ast \<Rightarrow> 'a nstate \<Rightarrow> bool"
+definition proc_body_satisfies_spec :: "'a absval_ty_fun \<Rightarrow> 'struct_ty proc_context \<Rightarrow> var_context \<Rightarrow> 'a fun_interp \<Rightarrow> rtype_env \<Rightarrow> expr list \<Rightarrow> expr list \<Rightarrow> ast \<Rightarrow> 'a nstate \<Rightarrow> bool"
   where "proc_body_satisfies_spec A M \<Lambda> \<Gamma> \<Omega> pres posts ast ns \<equiv>
          expr_all_sat A \<Lambda> \<Gamma> \<Omega> ns pres \<longrightarrow> 
           (\<forall> bb cont state. (rtranclp (red_bigblock A M \<Lambda> \<Gamma> \<Omega> ast) (init_ast ast ns) (bb, cont, state)) \<longrightarrow> 
                     valid_configuration A \<Lambda> \<Gamma> \<Omega> posts bb cont state)"
 
-fun proc_all_pres :: "ast_procedure \<Rightarrow> expr list"
+fun proc_all_pres :: "'struct_ty procedure \<Rightarrow> expr list"
   where "proc_all_pres p = map fst (proc_pres p)"
 
-fun proc_checked_posts :: "ast_procedure \<Rightarrow> expr list"
+fun proc_checked_posts :: "'struct_ty procedure \<Rightarrow> expr list"
   where "proc_checked_posts p = map fst (filter (\<lambda>x. \<not> snd(x)) (proc_posts p))"
 
+(*
 fun proc_is_correct :: "'a absval_ty_fun \<Rightarrow> fdecls \<Rightarrow> vdecls \<Rightarrow> vdecls \<Rightarrow> axiom list \<Rightarrow> ast_procedure \<Rightarrow> bool"
   where 
     "proc_is_correct A fun_decls constants global_vars axioms proc =
@@ -241,42 +235,21 @@ fun proc_is_correct :: "'a absval_ty_fun \<Rightarrow> fdecls \<Rightarrow> vdec
             )
           )))
       | None \<Rightarrow> True)"
+*)
 
-(* TODO: Rework this! *)
 inductive syntactic_equiv :: "expr \<Rightarrow> expr \<Rightarrow> bool" (infixl "\<sim>" 40) 
   where
-    refl [simp]:   "a \<sim> a"
-  | neg_cong:      "a \<sim> b \<Longrightarrow> UnOp Not a \<sim> UnOp Not b"
-  | conj_cong:     "a1 \<sim> b1 \<Longrightarrow> a2 \<sim> b2 \<Longrightarrow> (a1 \<guillemotleft>And\<guillemotright> a2) \<sim> (b1 \<guillemotleft>And\<guillemotright> b2)"
-  | disj_cong:     "a1 \<sim> b1 \<Longrightarrow> a2 \<sim> b2 \<Longrightarrow> (a1 \<guillemotleft>Or\<guillemotright> a2) \<sim> (b1 \<guillemotleft>Or\<guillemotright> b2)"
-  | conj_commute:  "(a \<guillemotleft>And\<guillemotright> b) \<sim> (b \<guillemotleft>And\<guillemotright> a)"
-  | disj_commute:  "(a \<guillemotleft>Or\<guillemotright> b) \<sim> (b \<guillemotleft>Or\<guillemotright> a)"
-  | conj_assoc:    "(a \<guillemotleft>And\<guillemotright> b) \<guillemotleft>And\<guillemotright> c \<sim> a \<guillemotleft>And\<guillemotright> (b \<guillemotleft>And\<guillemotright> c)"
-  | disj_assoc:    "(a \<guillemotleft>Or\<guillemotright> b) \<guillemotleft>Or\<guillemotright> c \<sim> a \<guillemotleft>Or\<guillemotright> (b \<guillemotleft>Or\<guillemotright> c)"
-  | disj_conj:     "a \<guillemotleft>Or\<guillemotright> (b \<guillemotleft>And\<guillemotright> c) \<sim> (a \<guillemotleft>Or\<guillemotright> b) \<guillemotleft>And\<guillemotright> (a \<guillemotleft>Or\<guillemotright> c)"
-  | conj_disj:     "a \<guillemotleft>And\<guillemotright> (b \<guillemotleft>Or\<guillemotright> c) \<sim> (a \<guillemotleft>And\<guillemotright> b) \<guillemotleft>Or\<guillemotright> (a \<guillemotleft>And\<guillemotright> c)"
-  | de_morgan1:    "UnOp Not (a \<guillemotleft>And\<guillemotright> b) \<sim> (UnOp Not a) \<guillemotleft>Or\<guillemotright> (UnOp Not b)"
-  | de_morgan2:    "UnOp Not (a \<guillemotleft>Or\<guillemotright> b) \<sim> (UnOp Not a) \<guillemotleft>And\<guillemotright> (UnOp Not b)"
-  | neg_neg:       "UnOp Not (UnOp Not a) \<sim> a"
-  | tnd:           "a \<guillemotleft>Or\<guillemotright> (UnOp Not) a \<sim> (Lit (LBool True))"
-  | contr:         "a \<guillemotleft>And\<guillemotright> (UnOp Not) a \<sim> (Lit (LBool False))"
-  | disj_idem:     "a \<guillemotleft>Or\<guillemotright> a \<sim> a"
-  | conj_idem:     "a \<guillemotleft>And\<guillemotright> a \<sim> a"
-  | conj_True:     "a \<guillemotleft>And\<guillemotright> (Lit (LBool True)) \<sim> a"
-  | disj_True:     "a \<guillemotleft>Or\<guillemotright> (Lit (LBool True)) \<sim> (Lit (LBool True))"
-  | neg_lt:        "UnOp Not (a \<guillemotleft>Lt\<guillemotright> b) \<sim> (a \<guillemotleft>Ge\<guillemotright> b)"
-  | neg_gt1:        "UnOp Not (a \<guillemotleft>Gt\<guillemotright> b) \<sim> (a \<guillemotleft>Le\<guillemotright> b)"
-  | neg_gt2:        "UnOp Not (a \<guillemotleft>Gt\<guillemotright> b) \<sim> (b \<guillemotleft>Ge\<guillemotright> a)"
-  | neg_le:        "UnOp Not (a \<guillemotleft>Le\<guillemotright> b) \<sim> (a \<guillemotleft>Gt\<guillemotright> b)"
-  | neg_ge:        "UnOp Not (a \<guillemotleft>Ge\<guillemotright> b) \<sim> (a \<guillemotleft>Lt\<guillemotright> b)"
-  | neg_lt2:        "UnOp Not (a \<guillemotleft>Lt\<guillemotright> b) \<sim> (b \<guillemotleft>Le\<guillemotright> a)"
-  | neg_eq:        "UnOp Not (a \<guillemotleft>Eq\<guillemotright> b) \<sim> (a \<guillemotleft>Neq\<guillemotright> b)"
-  | neg_neq:       "UnOp Not (a \<guillemotleft>Neq\<guillemotright> b) \<sim> (a \<guillemotleft>Eq\<guillemotright> b)"
+    neg_refl:       "UnOp Not e1 \<sim> UnOp Not e1"
+  | neg_equiv1: "UnOp Not (Lit (LBool True)) \<sim> (Lit (LBool False))"
+  | neg_equiv2: "UnOp Not (Lit (LBool False)) \<sim> (Lit (LBool True))"
+  | double_neg: "UnOp Not (UnOp Not e1) \<sim> e1"
+  | neg_eq:     "UnOp Not (a \<guillemotleft>Eq\<guillemotright> b) \<sim> (a \<guillemotleft>Neq\<guillemotright> b)"
+  | neg_neq:    "UnOp Not (a \<guillemotleft>Neq\<guillemotright> b) \<sim> (a \<guillemotleft>Eq\<guillemotright> b)"
+  | neg_lt:     "UnOp Not (a \<guillemotleft>Lt\<guillemotright> b) \<sim> (b \<guillemotleft>Le\<guillemotright> a)"
+  | neg_le:     "UnOp Not (a \<guillemotleft>Le\<guillemotright> b) \<sim> (b \<guillemotleft>Lt\<guillemotright> a)"
+  | neg_gt:     "UnOp Not (a \<guillemotleft>Gt\<guillemotright> b) \<sim> (b \<guillemotleft>Ge\<guillemotright> a)"
+  | neg_ge:     "UnOp Not (a \<guillemotleft>Ge\<guillemotright> b) \<sim> (b \<guillemotleft>Gt\<guillemotright> a)"
 
-(*
-definition semantic_equiv :: "expr \<Rightarrow> expr \<Rightarrow> bool" (infixl "\<approx>" 40) where
-  "exp1 \<approx> exp2 \<longleftrightarrow> (\<forall> A \<Lambda> \<Gamma> \<Omega> ns val. ((red_expr A \<Lambda> \<Gamma> \<Omega> exp1 ns val) = (red_expr A \<Lambda> \<Gamma> \<Omega> exp2 ns val)))"
-*)
 
 inductive ast_cfg_rel :: "expr option \<Rightarrow> cmd list \<Rightarrow> bigblock \<Rightarrow> cmd list \<Rightarrow> bool"
   where 
